theories/Open.v
@@ -26,65 +26,43 @@
 (* SOFTWARE, EVEN IF ADVISED OF THE POSSIBILITY OF SUCH DAMAGE.               *)
 (******************************************************************************)
 
-From Coq Require Import
-  Strings.String.
-From Em Require Import
-  Environment
-  Prelude
-  Stlc.Instantiation
-  Stlc.Spec
-  Stlc.Persistence
-  Stlc.Worlds.
+From Em Require Import Prelude Instantiation Spec Persistence Worlds.
 
-Module Sem.
+Module Open.
 
-  Definition Sem (A : Type) : TYPE :=
+  Definition Open (A : Type) : TYPE :=
     fun w => Assignment w → A.
 
   (* pure  :: a -> f a *)
-  Definition pure {A} (a : A) : Valid (Sem A) := fun _ _ => a.
+  Definition pure {A} (a : A) : Valid (Open A) := fun _ _ => a.
   #[global] Arguments pure {A} _ {w} ι/.
 
-  Definition fmap {A B} (f : A -> B) : ⊧ Sem A ⇢ Sem B :=
+  Definition fmap {A B} (f : A -> B) : ⊧ Open A ⇢ Open B :=
     fun w a ι => f (a ι).
   #[global] Arguments fmap {A B} _ {w} a ι/.
 
   (* ap :: f (a -> b) -> f a -> f b *)
-  Definition ap {A B : Type} : ⊧ Sem (A → B) ⇢ Sem A ⇢ Sem B :=
+  Definition ap {A B : Type} : ⊧ Open (A → B) ⇢ Open A ⇢ Open B :=
     fun w f a ι => f ι (a ι).
   #[global] Arguments ap {A B} [w] f a ι/.
 
-  #[export] Instance inst_sem {A} : Inst (Sem A) A :=
+  #[export] Instance inst_sem {A} : Inst (Open A) A :=
     fun w x ι => x ι.
   #[global] Arguments inst_sem {A} [w] x ι/.
 
-  #[export] Instance lift_sem {A} : Lift (Sem A) A :=
+  #[export] Instance lift_sem {A} : Lift (Open A) A :=
     pure.
 
-  #[export] Instance persistent_sem {A} : Persistent (Sem A) :=
+  #[export] Instance persistent_sem {A} : Persistent (Open A) :=
     fun Θ w0 t w1 θ ι => t (inst θ ι).
 
-  (* #[export] Instance persistlaws_sem {A} : PersistLaws (Sem A). *)
-  (* Proof. *)
-  (*   constructor. *)
-  (*   - intros. cbv [persist persistent_sem]. *)
-  (*     extensionality ι. now rewrite inst_refl. *)
-  (*   - intros. cbv [persist persistent_sem]. *)
-  (*     extensionality ι. now rewrite inst_trans. *)
-  (*   - intros. cbv [persist persistent_sem]. *)
-  (*     extensionality ι. f_equal. *)
-  (*     apply env.lookup_extensional. intros α αIn. *)
-  (*     change (inst (ṫy.var αIn) (inst θ1 ι) = inst (ṫy.var αIn) (inst θ2 ι)). *)
-  (*     rewrite <- ?inst_persist. f_equal. cbn. apply H. *)
-  (* Qed. *)
-
-  #[export] Instance inst_lift_sem {A} : InstLift (Sem A) A.
+  #[export] Instance inst_lift_sem {A} : InstLift (Open A) A.
   Proof. easy. Qed.
 
-  #[export] Instance inst_persist_sem {A} : InstPersist (Sem A) A.
+  #[export] Instance inst_persist_sem {A} : InstPersist (Open A) A.
   Proof. easy. Qed.
 
-  #[export] Instance persist_lift_sem {A} : PersistLift (Sem A) A.
+  #[export] Instance persist_lift_sem {A} : PersistLift (Open A) A.
   Proof. easy. Qed.
 
   Section InstLemmas.
@@ -93,11 +71,11 @@ Module Sem.
       inst (pure a) ι = a.
     Proof. reflexivity. Qed.
 
-    Lemma inst_fmap {A B} (f : A -> B) [w0] (a : Sem A w0) (ι : Assignment w0) :
+    Lemma inst_fmap {A B} (f : A -> B) [w0] (a : Open A w0) (ι : Assignment w0) :
       inst (fmap f a) ι = f (inst a ι).
     Proof. reflexivity. Qed.
 
-    Lemma inst_ap {A B} [w0] (f : Sem (A -> B) w0) (a : Sem A w0) (ι : Assignment w0) :
+    Lemma inst_ap {A B} [w0] (f : Open (A -> B) w0) (a : Open A w0) (ι : Assignment w0) :
       inst (ap f a) ι = (inst f ι) (inst a ι).
     Proof. reflexivity. Qed.
 
@@ -110,45 +88,45 @@ Module Sem.
       persist (pure a) θ = pure a.
     Proof. reflexivity. Qed.
 
-    Lemma persist_fmap {A B} (f : A -> B) [w0] (a : Sem A w0) [w1] (θ : Θ w0 w1) :
+    Lemma persist_fmap {A B} (f : A -> B) [w0] (a : Open A w0) [w1] (θ : Θ w0 w1) :
       persist (fmap f a) θ = fmap f (persist a θ).
     Proof. reflexivity. Qed.
 
-    Lemma persist_app {A B} [w0] (f : Sem (A -> B) w0) (a : Sem A w0) [w1] (θ : Θ w0 w1) :
+    Lemma persist_app {A B} [w0] (f : Open (A -> B) w0) (a : Open A w0) [w1] (θ : Θ w0 w1) :
       persist (ap f a) θ = ap (persist f θ) (persist a θ).
     Proof. reflexivity. Qed.
 
   End PersistLemmas.
 
-  Definition decode_ty : ⊧ Ṫy ⇢ Sem Ty := fun w t => inst t.
+  Definition decode_ty : ⊧ Ṫy ⇢ Open Ty := fun w t => inst t.
   #[global] Arguments decode_ty [w] _.
-  Definition decode_env : ⊧ Ėnv ⇢ Sem Env := fun w G => inst G.
+  Definition decode_env : ⊧ Ėnv ⇢ Open Env := fun w G => inst G.
   #[global] Arguments decode_env [w] _.
 
   Module notations.
 
-    Notation "f <$> a" := (@Sem.fmap _ _ f _ a) (at level 61, left associativity).
-    Notation "f <*> a" := (@Sem.ap _ _ _ f a) (at level 61, left associativity).
+    Notation "f <$> a" := (@Open.fmap _ _ f _ a) (at level 61, left associativity).
+    Notation "f <*> a" := (@Open.ap _ _ _ f a) (at level 61, left associativity).
 
   End notations.
 
-End Sem.
-Export (hints) Sem.
-Export Sem (Sem).
+End Open.
+Export (hints) Open.
+Export Open (Open).
 
-Notation Ėxp := (Sem Exp).
+Notation Ėxp := (Open Exp).
 Module ėxp.
-  Import Sem Sem.notations.
+  Import Open Open.notations.
 
   Set Implicit Arguments.
   Set Maximal Implicit Insertion.
 
   Definition var : ⊧ Const string ⇢ Ėxp :=
-    fun _ x => Sem.pure (exp.var x).
+    fun _ x => Open.pure (exp.var x).
   Definition true : ⊧ Ėxp :=
-    fun _ => Sem.pure exp.true.
+    fun _ => Open.pure exp.true.
   Definition false : ⊧ Ėxp :=
-    fun _ => Sem.pure exp.false.
+    fun _ => Open.pure exp.false.
   Definition ifte : ⊧ Ėxp ⇢ Ėxp ⇢ Ėxp ⇢ Ėxp :=
     fun _ e1 e2 e3 => exp.ifte <$> e1 <*> e2 <*> e3.
   Definition absu : ⊧ Const string ⇢ Ėxp ⇢ Ėxp :=
