theories/Composition.v
@@ -1,0 +1,148 @@
+(******************************************************************************)
+(* Copyright (c) 2023 Denis Carnier, Steven Keuchel                           *)
+(* All rights reserved.                                                       *)
+(*                                                                            *)
+(* Redistribution and use in source and binary forms, with or without         *)
+(* modification, are permitted provided that the following conditions are     *)
+(* met:                                                                       *)
+(*                                                                            *)
+(* 1. Redistributions of source code must retain the above copyright notice,  *)
+(*    this list of conditions and the following disclaimer.                   *)
+(*                                                                            *)
+(* 2. Redistributions in binary form must reproduce the above copyright       *)
+(*    notice, this list of conditions and the following disclaimer in the     *)
+(*    documentation and/or other materials provided with the distribution.    *)
+(*                                                                            *)
+(* THIS SOFTWARE IS PROVIDED BY THE COPYRIGHT HOLDERS AND CONTRIBUTORS        *)
+(* "AS IS" AND ANY EXPRESS OR IMPLIED WARRANTIES, INCLUDING, BUT NOT LIMITED  *)
+(* TO, THE IMPLIED WARRANTIES OF MERCHANTABILITY AND FITNESS FOR A PARTICULAR *)
+(* PURPOSE ARE DISCLAIMED. IN NO EVENT SHALL THE COPYRIGHT HOLDER OR          *)
+(* CONTRIBUTORS BE LIABLE FOR ANY DIRECT, INDIRECT, INCIDENTAL, SPECIAL,      *)
+(* EXEMPLARY, OR CONSEQUENTIAL DAMAGES (INCLUDING, BUT NOT LIMITED TO,        *)
+(* PROCUREMENT OF SUBSTITUTE GOODS OR SERVICES; LOSS OF USE, DATA, OR         *)
+(* PROFITS; OR BUSINESS INTERRUPTION) HOWEVER CAUSED AND ON ANY THEORY OF     *)
+(* LIABILITY, WHETHER IN CONTRACT, STRICT LIABILITY, OR TORT (INCLUDING       *)
+(* NEGLIGENCE OR OTHERWISE) ARISING IN ANY WAY OUT OF THE USE OF THIS         *)
+(* SOFTWARE, EVEN IF ADVISED OF THE POSSIBILITY OF SUCH DAMAGE.               *)
+(******************************************************************************)
+
+From Coq Require Import
+  extraction.ExtrHaskellBasic
+  extraction.ExtrHaskellNatInt
+  extraction.ExtrHaskellString
+  Lists.List
+  Strings.String.
+From iris Require Import bi.interface bi.derived_laws proofmode.tactics.
+From Em Require Import BaseLogic Gen.Synthesise PrenexConversion Spec Unification
+  Prefix
+  Environment
+  Gen.Synthesise
+  Instantiation
+  Monad.Free
+  Monad.Interface
+  Persistence
+  Prelude
+  Open
+  Spec
+  Worlds.
+
+Import option.notations.
+Import Pred Pred.Acc.
+Import ListNotations.
+
+Definition run {A} `{Persistent A} (m : Free A world.nil) :
+  option { w & A w } :=
+  '(existT w1 (θ1 , (xs , a))) <- (prenex m) ;;
+  '(existT w2 (θ2 , _))        <- solve xs ;;
+  Some (existT w2 (persist a θ2)).
+
+Definition reconstruct (Γ : Env) (e : Exp) :
+  option { w & Ṫy w * Ėxp w }%type :=
+  run (generate e (lift Γ)).
+
+Definition infer (e : Exp) :
+  option { w & Ṫy w }%type :=
+  match reconstruct empty e with
+  | Some (existT w (t,e)) => Some (existT w t)
+  | None => None
+  end.
+
+Definition reconstruct_grounded (Γ : Env) (e : Exp) : option (Ty * Exp) :=
+  '(existT w te) <- reconstruct Γ e ;;
+  Some (inst te (grounding w)).
+
+Definition reconstruct_closed (e : Exp) : option (Ty * Exp) :=
+  '(existT w te) <- reconstruct empty e ;;
+  Some (inst te (grounding w)).
+
+Section Examples.
+  Definition examples :=
+    List.map infer
+      [ exp.absu "x" (exp.var "x");
+        exp.absu "x" (exp.absu "y" (exp.var "x"))
+      ].
+
+  Arguments ṫy.var {w}%world_scope α%string_scope {αIn}.
+  Import world.notations.
+  Notation "( x , .. , y )" := (snoc .. (snoc nil x) .. y) : world_scope.
+End Examples.
+
+(* Extraction Inline world.view. *)
+Extraction Language Haskell.
+Extraction Inline
+  Bool.Bool.iff_reflect
+  Environment.env.view
+  Init.Datatypes.nat_rec
+  Init.Logic.False_rec
+  Init.Logic.and_rec
+  Init.Logic.and_rect
+  Init.Logic.eq_rec_r
+  Unification.atrav
+  Unification.flex
+  Unification.loeb
+  Unification.remove_acc_rect
+  Unification.varview
+  Worlds.Box
+  Worlds.Impl
+  Worlds.Impl
+  Worlds.Valid
+  Worlds.lk
+  Worlds._4
+  Worlds.world.view
+  stdpp.base.fmap
+  stdpp.gmap.gmap_fmap
+  stdpp.option.option_fmap.
+
+Extract Inductive reflect => "Prelude.Bool" [ "Prelude.True" "Prelude.False" ].
+
+Extract Inlined Constant Init.Datatypes.fst => "Prelude.fst".
+Extract Inlined Constant Init.Datatypes.snd => "Prelude.snd".
+
+Extraction "Infer" examples.
+
+Definition algorithmic_typing (Γ : Env) (e : Exp) (τ : Ty) (e' : Exp) : Prop :=
+  match reconstruct Γ e with
+  | Some (existT w1 (τ1, e1)) =>
+      exists ι : Assignment w1, inst τ1 ι = τ /\ inst e1 ι = e'
+  | None => False
+  end.
+
+Lemma correctness (Γ : Env) (e : Exp) (τ : Ty) (e' : Exp) :
+  algorithmic_typing Γ e τ e' <-> tpb Γ e τ e'.
+Proof.
+  generalize (generate_correct (M := Free) (w:=world.nil)
+                (lift Γ) e (lift τ) (lift e')).
+  unfold TPB_algo, algorithmic_typing, reconstruct, run.
+  rewrite <- prenex_correct. destruct prenex as [(w1 & θ1 & C & t1 & e1)|]; cbn.
+  - rewrite <- (solve_correct C).
+    destruct (solve C) as [(w2 & θ2 & [])|]; predsimpl.
+    + rewrite Acc.and_wp_l. predsimpl. unfold Acc.wp; pred_unfold.
+      intros HG. rewrite (HG env.nil). clear HG. split.
+      * intros (ι2 & Heq1 & Heq2). exists (inst θ2 ι2).
+        split; [now destruct (env.view (inst θ1 (inst θ2 ι2)))|].
+        exists ι2. now subst.
+      * intros (ι1 & Heq1 & ι2 & Heq2 & Heq3 & Heq4).
+        exists ι2. now subst.
+    + pred_unfold. intros HE. now specialize (HE env.nil).
+  - pred_unfold. intros HE. now specialize (HE env.nil).
+Qed.
