theories/Gen/Bidirectional.v
@@ -1,0 +1,235 @@
+(******************************************************************************)
+(* Copyright (c) 2023 Denis Carnier, Steven Keuchel                           *)
+(* All rights reserved.                                                       *)
+(*                                                                            *)
+(* Redistribution and use in source and binary forms, with or without         *)
+(* modification, are permitted provided that the following conditions are     *)
+(* met:                                                                       *)
+(*                                                                            *)
+(* 1. Redistributions of source code must retain the above copyright notice,  *)
+(*    this list of conditions and the following disclaimer.                   *)
+(*                                                                            *)
+(* 2. Redistributions in binary form must reproduce the above copyright       *)
+(*    notice, this list of conditions and the following disclaimer in the     *)
+(*    documentation and/or other materials provided with the distribution.    *)
+(*                                                                            *)
+(* THIS SOFTWARE IS PROVIDED BY THE COPYRIGHT HOLDERS AND CONTRIBUTORS        *)
+(* "AS IS" AND ANY EXPRESS OR IMPLIED WARRANTIES, INCLUDING, BUT NOT LIMITED  *)
+(* TO, THE IMPLIED WARRANTIES OF MERCHANTABILITY AND FITNESS FOR A PARTICULAR *)
+(* PURPOSE ARE DISCLAIMED. IN NO EVENT SHALL THE COPYRIGHT HOLDER OR          *)
+(* CONTRIBUTORS BE LIABLE FOR ANY DIRECT, INDIRECT, INCIDENTAL, SPECIAL,      *)
+(* EXEMPLARY, OR CONSEQUENTIAL DAMAGES (INCLUDING, BUT NOT LIMITED TO,        *)
+(* PROCUREMENT OF SUBSTITUTE GOODS OR SERVICES; LOSS OF USE, DATA, OR         *)
+(* PROFITS; OR BUSINESS INTERRUPTION) HOWEVER CAUSED AND ON ANY THEORY OF     *)
+(* LIABILITY, WHETHER IN CONTRACT, STRICT LIABILITY, OR TORT (INCLUDING       *)
+(* NEGLIGENCE OR OTHERWISE) ARISING IN ANY WAY OUT OF THE USE OF THIS         *)
+(* SOFTWARE, EVEN IF ADVISED OF THE POSSIBILITY OF SUCH DAMAGE.               *)
+(******************************************************************************)
+
+From stdpp Require Import base gmap.
+From iris Require Import proofmode.tactics.
+From Em Require Import BaseLogic Monad.Interface.
+
+Import Pred Pred.notations Pred.proofmode world.notations.
+
+Set Implicit Arguments.
+
+#[local] Notation "s [ ζ ]" :=
+  (persist s ζ)
+    (at level 7, left associativity,
+      format "s [ ζ ]").
+
+Section Generator.
+  Import MonadNotations.
+
+  Context {Θ} {reflΘ : Refl Θ} {stepΘ : Step Θ} {transΘ : Trans Θ}
+    {reflTransΘ : ReflTrans Θ} {lkReflΘ : LkRefl Θ} {lkTransΘ : LkTrans Θ}
+    {lkStepΘ : LkStep Θ}.
+  Context {M} {pureM : Pure M} {bindM : Bind Θ M} {tcM : TypeCheckM M} .
+
+  Fixpoint check (e : Exp) : ⊧ Ėnv ⇢ Ṫy ⇢ M Ėxp :=
+    fun w Γ τ =>
+      match e with
+      | exp.var x =>
+          match lookup x Γ with
+          | Some τ' => _ <- assert τ τ' ;;
+                       pure (ėxp.var x)
+          | None    => fail
+          end
+      | exp.true  =>
+          _ <- assert τ ṫy.bool ;;
+          pure ėxp.true
+      | exp.false =>
+          _ <- assert τ ṫy.bool ;;
+          pure ėxp.false
+      | exp.ifte e1 e2 e3 =>
+          e1' <- check e1 Γ ṫy.bool ;;
+          e2' <- check e2 Γ[_] τ[_] ;;
+          e3' <- check e3 Γ[_] τ[_] ;;
+          pure (ėxp.ifte e1'[_] e2'[_] e3')
+      | exp.absu x e =>
+          t1  <- pick ;;
+          t2  <- pick ;;
+          _   <- assert τ[_] (ṫy.func t1[_] t2) ;;
+          e'  <- check e (Γ[_] ,, x∷t1[_]) t2[_] ;;
+          pure (ėxp.abst x t1[_] e')
+      | exp.abst x t1 e =>
+          τ2  <- pick ;;
+          _   <- assert τ[_] (ṫy.func (lift t1) τ2) ;;
+          e'  <- check e (Γ[_] ,, x∷lift t1) τ2[_] ;;
+          pure (ėxp.abst x (lift t1) e')
+      | exp.app e1 e2 =>
+         '(τ2,e2') <- synth e2 Γ ;;
+         e1'       <- check e1 Γ[_] (ṫy.func τ2 τ[_]) ;;
+         pure (ėxp.app e1' e2'[_])
+      end
+  with synth (e : Exp) : ⊧ Ėnv ⇢ M (Ṫy * Ėxp) :=
+    fun w Γ =>
+      match e with
+      | exp.var x =>
+          match lookup x Γ with
+          | Some t => pure (t , ėxp.var x)
+          | None   => fail
+          end
+      | exp.true  => pure (ṫy.bool, ėxp.true)
+      | exp.false => pure (ṫy.bool, ėxp.false)
+      | exp.ifte e1 e2 e3 =>
+          e1'        <- check e1 Γ ṫy.bool ;;
+          '(τ,e2')   <- synth e2 Γ[_] ;;
+          e3'        <- check e3 Γ[_] τ ;;
+          pure (τ[_], ėxp.ifte e1'[_] e2'[_] e3')
+      | exp.absu x e =>
+          t1         <- pick ;;
+          '(t2,e')   <- synth e (insert (M := Ėnv _) x t1 Γ[_]) ;;
+          pure (ṫy.func t1[_] t2, ėxp.abst x t1[_] e')
+      | exp.abst x t1 e =>
+          '(t2,e')   <- synth e (insert (M := Ėnv _) x (lift t1) Γ) ;;
+          pure (ṫy.func (lift t1) t2, ėxp.abst x (lift t1) e')
+      | exp.app e1 e2 =>
+          '(tf, e1') <- synth e1 Γ ;;
+          τ1         <- pick ;;
+          τ2         <- pick ;;
+          _          <- assert tf[_] (ṫy.func τ1[_] τ2) ;;
+          e2'        <- check e2 Γ[_] τ1[_] ;;
+          pure (τ2[_], ėxp.app e1'[_] e2')
+      end.
+
+  Import Pred Pred.notations.
+  Import Pred.proofmode.
+  Import iris.proofmode.tactics.
+  Open Scope pred_scope.
+
+  Context {wpM : WeakestPre Θ M} {wlpM : WeakestLiberalPre Θ M}
+    {tcLogicM : TypeCheckLogicM Θ M}.
+
+  Definition TPB_algo : ⊧ Ėnv ⇢ Const Exp ⇢ Ṫy ⇢ Ėxp ⇢ Pred :=
+    fun w0 G0 e t0 e0 =>
+    WP (synth e G0)
+      (fun w1 (θ1 : Θ w0 w1) '(t1,e1) =>
+         t0[θ1] =ₚ t1 /\ₚ e0[θ1] =ₚ e1).
+
+  Ltac wlpauto :=
+    repeat
+      (repeat wpsimpl;
+       try
+         match goal with
+         | H: _ /\ _ |- _ => destruct H
+         | IH: forall w G, bi_emp_valid (WLP (synth ?e G) _)
+           |- environments.envs_entails _ (WLP (synth ?e ?G) _) =>
+             iApply (wlp_mono' $! (IH _ G));
+             iIntros (?w ?θ) "!>"; iIntros ([?t ?e']) "#?"
+         | IH: forall w G τ, bi_emp_valid (WLP (check ?e G τ) _)
+           |- environments.envs_entails _ (WLP (check ?e ?G ?τ) _) =>
+             iApply (wlp_mono' $! (IH _ G τ));
+             iIntros (?w ?θ) "!>"; iIntros (?e') "#?"
+         | |- environments.envs_entails _ (TPB _ _ _ _) =>
+             predsimpl;
+             iStopProof;
+             pred_unfold;
+             intuition (subst; econstructor; eauto; fail)
+         end).
+
+  Lemma sound_aux e :
+      (∀ w (G : Ėnv w) (t : Ṫy w),
+          ⊢ WLP (check e G t) (fun _ θ ee => G[θ] |--ₚ e; t[θ] ~> ee)) /\
+      (∀ w (G : Ėnv w),
+          ⊢ WLP (synth e G) (fun _ θ '(t,ee) => G[θ] |--ₚ e; t ~> ee)).
+  Proof.
+    induction e; cbn; (split; [intros w G τ|intros w G]); iStartProof; wlpauto.
+    - destruct lookup eqn:HGx; wlpauto. iStopProof; pred_unfold.
+      intros ->. constructor. now rewrite lookup_inst HGx.
+    - destruct lookup eqn:HGx; wlpauto. iStopProof; pred_unfold.
+      constructor. now rewrite lookup_inst HGx.
+  Qed.
+
+  Lemma sound (e : Exp) (w0 : World) (G0 : Ėnv w0) t0 e0 :
+    TPB_algo G0 e t0 e0 ⊢ₚ G0 |--ₚ e; t0 ~> e0.
+  Proof.
+    iStartProof. rewrite wand_is_impl. iApply wp_impl.
+    destruct (@sound_aux e) as [_ Hsound].
+    iApply (wlp_mono' $! (@Hsound w0 G0)).
+    iIntros "%w1 %θ1 !>" ([t e']) "HT". predsimpl.
+    iStopProof; pred_unfold. intros HT Heq1 Heq2. now subst.
+  Qed.
+
+  Ltac wpauto :=
+    repeat
+      (repeat wpsimpl;
+       try
+         match goal with
+         | H: _ /\ _ |- _ => destruct H
+         | IH: forall (w : World) (G : Ėnv w) (t : Ṫy w),
+             bi_emp_valid (bi_impl _ (bi_impl _ (WP (check ?e G t) _)))
+             |- environments.envs_entails _ (WP (check ?e ?G ?t) _) =>
+             iPoseProof (IH _ G t with "[] []") as "-#IH"; clear IH;
+             [ | | iApply (wp_mono' with "IH");
+                   iIntros (?w ?θ) "!>"; iIntros (?e') "#?"
+             ]
+         | IH: forall _ G,
+             bi_emp_valid (bi_impl _ (WP (synth ?e G) _))
+             |- environments.envs_entails _ (WP (synth ?e ?G) _) =>
+             iPoseProof (IH _ G with "[]") as "-#IH"; clear IH;
+             [| iApply (wp_mono' with "IH");
+                iIntros (?w ?θ) "!>";
+                iIntros ((?t & ?e')) "(#? & #?)"
+             ]
+         end).
+
+  Lemma complete_aux {G e t ee} (T : G |-- e ∷ t ~> ee) :
+    (∀ w0 (G0 : Ėnv w0) (t0 : Ṫy w0),
+      ⊢ lift G =ₚ G0 ->ₚ lift t =ₚ t0 ->ₚ
+        WP (check e G0 t0) (fun _ _ e' => Open.pure ee =ₚ e')%P) /\
+    (∀ w0 (G0 : Ėnv w0),
+      ⊢ lift G =ₚ G0 →
+        WP (synth e G0) (fun _ _ '(t',e') => lift t =ₚ t' /\ₚ Open.pure ee =ₚ e')%P).
+  Proof.
+    induction T; cbn; (split; [intros ? G0 ?|intros ? G0]); iStartProof; wpauto.
+    - destruct (G0 !! _) eqn:HGx; wpauto.
+      + iApply wp_assert. iSplit.
+        * iStopProof; pred_unfold. intros ? [-> ->].
+          rewrite lookup_inst HGx in H. now injection H.
+        * iIntros (?w ?θ) "!>"; wpauto.
+      + iStopProof; pred_unfold. intros ? []. subst.
+        rewrite lookup_inst HGx in H. now discriminate H.
+    - destruct (G0 !! _) eqn:HGx; wpauto; iStopProof; pred_unfold;
+        intros ? ->; rewrite lookup_inst HGx in H; cbn in H; congruence.
+  Qed.
+
+  Lemma complete (e : Exp) (w0 : World) (G0 : Ėnv w0) t0 e0 :
+    G0 |--ₚ e; t0 ~> e0 ⊢ₚ TPB_algo G0 e t0 e0.
+  Proof.
+    pred_unfold. intros ι HT.
+    destruct (complete_aux HT) as [_ Hcompl].
+    specialize (Hcompl _ G0). destruct Hcompl as [Hcompl].
+    specialize (Hcompl ι (MkEmp _)). pred_unfold.
+    rewrite inst_lift in Hcompl.
+    specialize (Hcompl eq_refl). revert Hcompl.
+    apply wp_mono. intros w1 θ1 ι1 <- [τ1 e1].
+    pred_unfold.
+  Qed.
+
+  Lemma correct {w} (Γ : Ėnv w) (e : Exp) (τ : Ṫy w) (e' : Ėxp w) :
+    Γ |--ₚ e; τ ~> e' ⊣⊢ₚ TPB_algo Γ e τ e'.
+  Proof. iSplit. iApply complete. iApply sound. Qed.
+
+End Generator.
