theories/Gen/Check.v
@@ -1,0 +1,176 @@
+(******************************************************************************)
+(* Copyright (c) 2023 Denis Carnier, Steven Keuchel                           *)
+(* All rights reserved.                                                       *)
+(*                                                                            *)
+(* Redistribution and use in source and binary forms, with or without         *)
+(* modification, are permitted provided that the following conditions are     *)
+(* met:                                                                       *)
+(*                                                                            *)
+(* 1. Redistributions of source code must retain the above copyright notice,  *)
+(*    this list of conditions and the following disclaimer.                   *)
+(*                                                                            *)
+(* 2. Redistributions in binary form must reproduce the above copyright       *)
+(*    notice, this list of conditions and the following disclaimer in the     *)
+(*    documentation and/or other materials provided with the distribution.    *)
+(*                                                                            *)
+(* THIS SOFTWARE IS PROVIDED BY THE COPYRIGHT HOLDERS AND CONTRIBUTORS        *)
+(* "AS IS" AND ANY EXPRESS OR IMPLIED WARRANTIES, INCLUDING, BUT NOT LIMITED  *)
+(* TO, THE IMPLIED WARRANTIES OF MERCHANTABILITY AND FITNESS FOR A PARTICULAR *)
+(* PURPOSE ARE DISCLAIMED. IN NO EVENT SHALL THE COPYRIGHT HOLDER OR          *)
+(* CONTRIBUTORS BE LIABLE FOR ANY DIRECT, INDIRECT, INCIDENTAL, SPECIAL,      *)
+(* EXEMPLARY, OR CONSEQUENTIAL DAMAGES (INCLUDING, BUT NOT LIMITED TO,        *)
+(* PROCUREMENT OF SUBSTITUTE GOODS OR SERVICES; LOSS OF USE, DATA, OR         *)
+(* PROFITS; OR BUSINESS INTERRUPTION) HOWEVER CAUSED AND ON ANY THEORY OF     *)
+(* LIABILITY, WHETHER IN CONTRACT, STRICT LIABILITY, OR TORT (INCLUDING       *)
+(* NEGLIGENCE OR OTHERWISE) ARISING IN ANY WAY OUT OF THE USE OF THIS         *)
+(* SOFTWARE, EVEN IF ADVISED OF THE POSSIBILITY OF SUCH DAMAGE.               *)
+(******************************************************************************)
+
+From stdpp Require Import base gmap.
+From iris Require Import proofmode.tactics.
+From Em Require Import BaseLogic Monad.Interface.
+
+Import Pred Pred.notations Pred.proofmode world.notations.
+
+Set Implicit Arguments.
+
+#[local] Notation "s [ ζ ]" :=
+  (persist s ζ)
+    (at level 7, left associativity,
+      format "s [ ζ ]").
+
+Section Generator.
+  Import MonadNotations.
+
+  Context {Θ} {reflΘ : Refl Θ} {stepΘ : Step Θ} {transΘ : Trans Θ}
+    {reflTransΘ : ReflTrans Θ} {lkReflΘ : LkRefl Θ} {lkTransΘ : LkTrans Θ}
+    {lkStepΘ : LkStep Θ}.
+  Context {M} {pureM : Pure M} {bindM : Bind Θ M} {tcM : TypeCheckM M} .
+
+  Definition check : Exp -> ⊧ Ėnv ⇢ Ṫy ⇢ M Ėxp :=
+    fix gen e {w} Γ τ :=
+      match e with
+      | exp.var x =>
+          match lookup x Γ with
+          | Some τ' => _ <- assert τ τ' ;;
+                       pure (ėxp.var x)
+          | None    => fail
+          end
+      | exp.true  =>
+          _ <- assert τ ṫy.bool ;;
+          pure ėxp.true
+      | exp.false =>
+          _ <- assert τ ṫy.bool ;;
+          pure ėxp.false
+      | exp.ifte e1 e2 e3 =>
+          e1' <- gen e1 Γ ṫy.bool ;;
+          e2' <- gen e2 Γ[_] τ[_] ;;
+          e3' <- gen e3 Γ[_] τ[_] ;;
+          pure (ėxp.ifte e1'[_] e2'[_] e3')
+      | exp.absu x e =>
+          t1  <- pick ;;
+          t2  <- pick ;;
+          e'  <- gen e (Γ[_] ,, x∷t1[_]) t2 ;;
+          _   <- assert (τ[_]) (ṫy.func t1[_] t2[_]) ;;
+          pure (ėxp.abst x t1[_] e'[_])
+      | exp.abst x t1 e =>
+          t2  <- pick ;;
+          e'  <- gen e (Γ[_] ,, x∷lift t1) t2 ;;
+          _   <- assert (τ[_]) (ṫy.func (lift t1) t2[_]) ;;
+          pure (ėxp.abst x (lift t1) e'[_])
+      | exp.app e1 e2 =>
+          t1  <- pick ;;
+          e1' <- gen e1 Γ[_] (ṫy.func t1 τ[_]) ;;
+          e2' <- gen e2 Γ[_] t1[_] ;;
+          pure (ėxp.app e1'[_] e2')
+      end.
+
+  Definition synth (e : Exp) :
+    ⊧ Ėnv ⇢ M (Prod Ṫy Ėxp) :=
+    fun w G =>
+      τ  <- pick ;;
+      e' <- check e G[_] τ ;;
+      pure (τ[_] , e').
+
+  Import Pred.proofmode.
+  Import iris.proofmode.tactics.
+  Open Scope pred_scope.
+  Import Pred Pred.notations.
+  (* Import (notations) Open. *)
+
+  Context {wpM : WeakestPre Θ M} {wlpM : WeakestLiberalPre Θ M}
+    {tcLogicM : TypeCheckLogicM Θ M}.
+
+  Definition TPB_algo : ⊧ Ėnv ⇢ Const Exp ⇢ Ṫy ⇢ Ėxp ⇢ Pred :=
+    fun w0 G0 e τ0 e0 => WP (check e G0 τ0) (fun _ θ1 e1 => e0[θ1] =ₚ e1).
+
+  Ltac wlpauto := repeat (repeat wpsimpl; try
+    match goal with
+    | IH: ∀ w G τ, bi_emp_valid (WLP (check ?e G τ) _)
+      |- environments.envs_entails _ (WLP (check ?e ?G ?τ) _) =>
+        iApply (wlp_mono' $! (IH _ G τ));
+        iIntros (?w ?θ) "!>"; iIntros (?e') "#?"
+    | |- environments.envs_entails _ (TPB _ _ _ _) =>
+        predsimpl; iStopProof; pred_unfold;
+        intuition (subst; econstructor; eauto; fail)
+    end).
+
+  Lemma sound_aux e :
+    ∀ w (G : Ėnv w) (t : Ṫy w),
+      ⊢ WLP (check e G t) (fun w1 θ ee => G[θ] |--ₚ e; t[θ] ~> ee).
+  Proof.
+    induction e; cbn; intros w G τ; iStartProof; wlpauto.
+    destruct lookup eqn:HGx; wlpauto. iStopProof; pred_unfold.
+    intros ->. constructor. now rewrite lookup_inst HGx.
+  Qed.
+
+  Lemma sound (e : Exp) (w0 : World) (G0 : Ėnv w0) t0 e0 :
+    TPB_algo G0 e t0 e0 ⊢ₚ G0 |--ₚ e; t0 ~> e0.
+  Proof.
+    iStartProof. rewrite wand_is_impl. rewrite -wp_impl.
+    iApply (wlp_mono' $! (@sound_aux e w0 G0 t0)).
+    iIntros "%w1 %θ1 !>" (e') "HT". iStopProof. pred_unfold.
+    intros HT Heq. now subst.
+  Qed.
+
+  Ltac wpauto := repeat (repeat wpsimpl; try
+    match goal with
+    | IH: ∀ w (G : Ėnv w) (t : Ṫy w),
+        bi_emp_valid (bi_impl _ (bi_impl _ (WP (check ?e G t) _)))
+        |- environments.envs_entails _ (WP (check ?e ?G ?t) _) =>
+        iPoseProof (IH _ G t with "[] []") as "-#IH"; clear IH;
+        [ | | iApply (wp_mono' with "IH");
+              iIntros (?w ?θ) "!>"; iIntros (?e') "#?"
+        ]
+    end).
+
+  Lemma complete_aux {G e t ee} (T : G |-- e ∷ t ~> ee) :
+    ∀ w0 (G0 : Ėnv w0) (t0 : Ṫy w0),
+      ⊢ lift G =ₚ G0 ->ₚ lift t =ₚ t0 ->ₚ
+      WP (check e G0 t0) (fun _ _ e' => Open.pure ee =ₚ e')%P.
+  Proof.
+    induction T; cbn; intros w0 G0 t0; iStartProof; wpauto.
+    destruct (G0 !! _) eqn:HGx; wpauto.
+    + iApply wp_assert. iSplit.
+      * iStopProof; pred_unfold. intros ? [-> ->].
+        rewrite lookup_inst HGx in H. now injection H.
+      * iIntros (?w ?θ) "!>"; wpauto.
+    + iStopProof; pred_unfold. intros ? []. subst.
+      rewrite lookup_inst HGx in H. now discriminate H.
+  Qed.
+
+  Lemma complete (e : Exp) w0 (G0 : Ėnv w0) t0 e0 :
+    G0 |--ₚ e; t0 ~> e0 ⊢ₚ TPB_algo G0 e t0 e0.
+  Proof.
+    unfold TPB_algo. pred_unfold. intros ι HT.
+    pose proof (complete_aux HT G0 t0) as [Hcompl].
+    specialize (Hcompl ι (MkEmp _)). pred_unfold.
+    rewrite ?inst_lift in Hcompl. specialize (Hcompl eq_refl eq_refl).
+    revert Hcompl. apply wp_mono. intros w1 θ1 e1 <-. predsimpl.
+  Qed.
+
+  Lemma correct {w} (Γ : Ėnv w) (e : Exp) (τ : Ṫy w) (e' : Ėxp w) :
+    Γ |--ₚ e; τ ~> e' ⊣⊢ₚ TPB_algo Γ e τ e'.
+  Proof. iSplit. iApply complete. iApply sound. Qed.
+
+End Generator.
