theories/Monad/Solved.v
@@ -1,0 +1,92 @@
+(******************************************************************************)
+(* Copyright (c) 2023 Denis Carnier, Steven Keuchel                           *)
+(* All rights reserved.                                                       *)
+(*                                                                            *)
+(* Redistribution and use in source and binary forms, with or without         *)
+(* modification, are permitted provided that the following conditions are     *)
+(* met:                                                                       *)
+(*                                                                            *)
+(* 1. Redistributions of source code must retain the above copyright notice,  *)
+(*    this list of conditions and the following disclaimer.                   *)
+(*                                                                            *)
+(* 2. Redistributions in binary form must reproduce the above copyright       *)
+(*    notice, this list of conditions and the following disclaimer in the     *)
+(*    documentation and/or other materials provided with the distribution.    *)
+(*                                                                            *)
+(* THIS SOFTWARE IS PROVIDED BY THE COPYRIGHT HOLDERS AND CONTRIBUTORS        *)
+(* "AS IS" AND ANY EXPRESS OR IMPLIED WARRANTIES, INCLUDING, BUT NOT LIMITED  *)
+(* TO, THE IMPLIED WARRANTIES OF MERCHANTABILITY AND FITNESS FOR A PARTICULAR *)
+(* PURPOSE ARE DISCLAIMED. IN NO EVENT SHALL THE COPYRIGHT HOLDER OR          *)
+(* CONTRIBUTORS BE LIABLE FOR ANY DIRECT, INDIRECT, INCIDENTAL, SPECIAL,      *)
+(* EXEMPLARY, OR CONSEQUENTIAL DAMAGES (INCLUDING, BUT NOT LIMITED TO,        *)
+(* PROCUREMENT OF SUBSTITUTE GOODS OR SERVICES; LOSS OF USE, DATA, OR         *)
+(* PROFITS; OR BUSINESS INTERRUPTION) HOWEVER CAUSED AND ON ANY THEORY OF     *)
+(* LIABILITY, WHETHER IN CONTRACT, STRICT LIABILITY, OR TORT (INCLUDING       *)
+(* NEGLIGENCE OR OTHERWISE) ARISING IN ANY WAY OUT OF THE USE OF THIS         *)
+(* SOFTWARE, EVEN IF ADVISED OF THE POSSIBILITY OF SUCH DAMAGE.               *)
+(******************************************************************************)
+
+From iris Require Import proofmode.tactics.
+From Em Require Import Monad.Interface Unification.
+
+Import Pred Pred.Acc Pred.proofmode Par world.notations.
+
+Definition Solved A :=
+  Option (Diamond Par A).
+
+#[export] Instance pure_solved : Pure Solved :=
+  fun A w a => Some (existT w (refl, a)).
+
+#[export] Instance bind_solved : Bind Par Solved :=
+  fun A B w m f =>
+    match m with
+    | Some (existT w1 (θ1, a1)) =>
+        match f w1 θ1 a1 with
+        | Some (existT w2 (θ2, b2)) =>
+            Some (existT w2 (θ1 ⊙ θ2, b2))
+        | None => None
+        end
+    | None => None
+    end.
+
+#[export] Instance tcm_solved : TypeCheckM Solved :=
+  {| assert w τ1 τ2 :=
+      match mgu τ1 τ2 with
+      | Some (existT x (a0, _)) => Some (existT x (Par.of a0, ()))
+      | None => None
+      end;
+     pick w := let α := world.fresh w in
+               Some (existT (w ▻ α) (step, ṫy.var world.in_zero));
+     Interface.fail A w := None;
+  |}.
+
+#[export] Instance wp_solved : WeakestPre Par Solved :=
+  fun A w o Q => wp_option o (fun d => wp_diamond d Q).
+#[export] Instance wlp_solved : WeakestLiberalPre Par Solved :=
+  fun A w o Q => wlp_option o (fun d => wlp_diamond d Q).
+
+#[export] Instance tcmlogic_solved : TypeCheckLogicM Par Solved.
+Proof.
+  constructor; intros; predsimpl.
+  - destruct m as [(w1 & θ1 & a1)|]; predsimpl.
+    destruct f as [(w2 & θ2 & b2)|]; predsimpl.
+  - rewrite <- mgu_correct. destruct mgu as [(w1 & θ1 & [])|]; predsimpl.
+    rewrite -Acc.wp_par_of. iIntros "[Hwp HQ]". iRevert "Hwp".
+    iApply Acc.wp_mono. iIntros "!> _". iMod "HQ". now rewrite trans_refl_r.
+  - rewrite <- (intro_wp_step τ). iIntros "#HQ !> #Heq". iMod "HQ".
+    rewrite trans_refl_r. iApply "HQ". now iModIntro.
+  - destruct m as [(w1 & θ1 & a1)|]; predsimpl.
+    iIntros "PQ". iApply Acc.wp_mono. iModIntro.
+    iMod "PQ". now rewrite trans_refl_r.
+  - destruct m as [(w1 & θ1 & a1)|]; predsimpl.
+    destruct f as [(w2 & θ2 & b2)|]; predsimpl.
+  - rewrite <- mgu_correct. destruct mgu as [(w1 & θ1 & [])|]; predsimpl.
+    rewrite -Acc.wp_par_of Acc.wp_impl. predsimpl. iIntros "HQ !>".
+    rewrite persist_update. iMod "HQ". now rewrite trans_refl_r.
+  - iIntros "HQ !>". iMod "HQ". rewrite trans_refl_r. iApply "HQ".
+  - destruct m as [(w1 & θ1 & a1)|]; predsimpl.
+    iIntros "PQ". iApply Acc.wlp_mono. iModIntro.
+    iMod "PQ". now rewrite trans_refl_r.
+  - destruct m as [(w1 & θ1 & a1)|]; predsimpl.
+    rewrite Acc.wp_impl. predsimpl.
+Qed.
